\todo{intro simplification}

\section{Type Automata}
\todo{intro type automata}

\section{Encoding}
\todo{explain encoding}

\begin{figure}[!htb]
    \begin{center}
    \begin{framed}
    \begin{minipage}[t]{0.95\columnwidth}
    \begin{mathpar}    
        \inferrule[Type Automata]{}{
            \Sigma_F ::= \{d, r, dh, rh, t, e \} \\
            T ::= \{ \functp, \handtp, \booltp, \dirttp\} \\
            \Sigma ::= V^+ \cup V^- \cup \Sigma_F^+ \cup \Sigma_F^- \cup T^+ \cup T^-\\ 
            E ::= \emptyset\, |\, \epsilon\, |\, \Sigma\, |\, E + E\, |\, E . E
        }\\

        \inferrule[]{}{
            \enctype^+(\functp) = \functp^+ \\
            \enctype^+(\handtp) = \handtp^+ \\
            \enctype^+(\booltp) = \booltp^+ \\
            \enctype^+(\dirttp) = \dirttp^+ \\
            \enctype^-(\functp) = \functp^- \\
            \enctype^-(\handtp) = \handtp^- \\
            \enctype^-(\booltp) = \booltp^- \\
            \enctype^-(\dirttp) = \dirttp^-
        }

    \end{mathpar}
    \end{minipage}

    \begin{minipage}[t]{0.475\columnwidth}
    \begin{mathpar}
        \inferrule[]{}{
            \enctype^+(\C) = \enctype^+(A \E \dirt) =\\ t^+ . \enctype^+(A) + e^+ . \enctype^+(\dirt) + \enctype^+(\dirttp)
        }\\

        \inferrule[]{}{
            \enctype^+(\alpha) = \alpha^+
        }\\

        \inferrule[]{}{
            \enctype^+(A_1 \union A_2) = \enctype^+(A_1) + \enctype^+(A_2)
        }\\

        \inferrule[]{}{
            \enctype^+(\bot) = \emptyset
        }\\

        \inferrule[]{}{
            \enctype^+(A \to \C) = d^+ . \enctype^-(A) +\\ r^+ . \enctype^+(\C) + \enctype^+(\functp)
        }\\

        \inferrule[]{}{
            \enctype^+(\C \hto \D) = dh^+ . \enctype^-(\C) +\\ rh^+ . \enctype^+(\D) + \enctype^+(\handtp)
        }\\

        \inferrule[]{}{
            \enctype^+(bool) = \enctype^+(\booltp)
        }\\
        
        \inferrule[]{}{
            \enctype^+(\rectype{A}) = \Omega^+_\alpha(A)^*. \enctype^+([\bot / \alpha]A)
        }\\
    
        \inferrule[]{}{
            \enctype^+(\op) = \optp{\op}^+
        }\\

        \inferrule[]{}{
            \enctype^+(\delta) = \delta^+
        }\\
    
        \inferrule[]{}{
            \enctype^+(\dirt_1 \union \dirt_2) = \enctype^+(\dirt_1) + \enctype^+(\dirt_2)
        }

    \end{mathpar}
    \end{minipage}
    \begin{minipage}[t]{0.475\columnwidth}
    \begin{mathpar}
        \inferrule[]{}{
            \enctype^-(\C) = \enctype^-(A \E \dirt) =\\ t^- . \enctype^-(A) + e^- . \enctype^-(\dirt) + \enctype^-(\dirttp)
        }\\

        \inferrule[]{}{
            \enctype^-(\alpha) = \alpha^-
        }\\

        \inferrule[]{}{
            \enctype^-(A_1 \intersection A_2) = \enctype^-(A_1) + \enctype^-(A_2)
        }\\

        \inferrule[]{}{
            \enctype^-(\top) = \emptyset
        }\\

        \inferrule[]{}{
            \enctype^-(A \to \C) = d^- . \enctype^+(A) +\\ r^- . \enctype^-(\C) + \enctype^-(\functp)
        }\\

        \inferrule[]{}{
            \enctype^-(\C \hto \D) = dh^- . \enctype^+(\C) +\\ rh^- . \enctype^-(\D) + \enctype^-(\handtp)
        }\\

        \inferrule[]{}{
            \enctype^-(bool) = \enctype^-(\booltp)
        }\\
        
        \inferrule[]{}{
            \enctype^-(\rectype{A}) = \Omega^-_\alpha(A)^*. \enctype^-([\top / \alpha]A)
        }\\
    
        \inferrule[]{}{
            \enctype^-(\op) = \optp{\op}^-
        }\\

        \inferrule[]{}{
            \enctype^-(\delta) = \delta^-
        }\\
    
        \inferrule[]{}{
            \enctype^-(\dirt_1 \intersection \dirt_2) = \enctype^-(\dirt_1) + \enctype^-(\dirt_2)
        }
    \end{mathpar}
    \end{minipage}

    \end{framed}
    \end{center}
\caption{Encoding types as type automata}\label{fig:automata:enc}
\end{figure}

\begin{figure}[!htb]
    \begin{center}
    \begin{framed}
    \begin{minipage}[t]{0.95\columnwidth}
    \begin{mathpar}    
        \inferrule[Type Automata]{}{
            \Sigma_F ::= \{d, r, dh, rh, t, e \} \\
            T ::= \{ \functp, \handtp, \booltp, \dirttp\} \\
            \Sigma ::= V^+ \cup V^- \cup \Sigma_F^+ \cup \Sigma_F^- \cup T^+ \cup T^-\\ 
            E ::= \emptyset\, |\, \epsilon\, |\, \Sigma\, |\, E + E\, |\, E . E
        }
    \end{mathpar}
    \end{minipage}

    \begin{minipage}[t]{0.475\columnwidth}
    \begin{mathpar}
        \inferrule[]{}{
            \Omega_\alpha^+(\C) = \Omega_\alpha^+(A \E \dirt) =\\ t^+ . \Omega_\alpha^+(A) + e^+ . \Omega_\alpha^+(\dirt)
        }\\

        \inferrule[]{}{
            \Omega_\alpha^+(\alpha) = \epsilon
        }\\

        \inferrule[]{}{
            \Omega_\alpha^+(\beta) = \emptyset
        }\\

        \inferrule[]{}{
            \Omega_\alpha^+(A_1 \union A_2) = \Omega_\alpha^+(A_1) + \Omega_\alpha^+(A_2)
        }\\

        \inferrule[]{}{
            \Omega_\alpha^+(\bot) = \emptyset
        }\\

        \inferrule[]{}{
            \Omega_\alpha^+(A \to \C) = d^+ . \Omega_\alpha^-(A) +\\ r^+ . \Omega_\alpha^+(\C)
        }\\

        \inferrule[]{}{
            \Omega_\alpha^+(\C \hto \D) = dh^+ . \Omega_\alpha^-(\C) + rh^+ . \Omega_\alpha^+(\D)
        }\\

        \inferrule[]{}{
            \Omega_\alpha^+(bool) = \emptyset
        }\\

        \inferrule[]{}{
            \Omega_\alpha^+(\op) = \emptyset
        }\\

        \inferrule[]{}{
            \Omega_\alpha^+(\delta) = \emptyset
        }\\

        \inferrule[]{}{
            \Omega_\alpha^+(\dirt_1 \union \dirt_2) = \Omega_\alpha^+(\dirt_1) + \Omega_\alpha^+(\dirt_2)
        }\\

        \inferrule[]{}{
            \Omega_\alpha^+(\rectype{A}) = \emptyset
        }\\

        \inferrule[]{}{
            \Omega_\alpha^-(\mu \beta . A) = \Omega^+_\beta(A)^*. \Omega_\alpha^+([\bot / \beta]A)
        }
    \end{mathpar}
    \end{minipage}
    \begin{minipage}[t]{0.475\columnwidth}
    \begin{mathpar}
        \inferrule[]{}{
            \Omega_\alpha^-(\C) = \Omega_\alpha^-(A \E \dirt) =\\ t^- . \Omega_\alpha^-(A) + e^- . \Omega_\alpha^-(\dirt)
        }\\

        \inferrule[]{}{
            \Omega_\alpha^-(\alpha) = \epsilon
        }\\

        \inferrule[]{}{
            \Omega_\alpha^-(\beta) = \emptyset
        }\\

        \inferrule[]{}{
            \Omega_\alpha^-(A_1 \union A_2) = \Omega_\alpha^-(A_1) + \Omega_\alpha^-(A_2)
        }\\

        \inferrule[]{}{
            \Omega_\alpha^-(\top) = \emptyset
        }\\

        \inferrule[]{}{
            \Omega_\alpha^-(A \to \C) = d^- . \Omega_\alpha^+(A) + r^- . \Omega_\alpha^-(\C)
        }\\

        \inferrule[]{}{
            \Omega_\alpha^-(\C \hto \D) = dh^- . \Omega_\alpha^+(\C) + rh^- . \Omega_\alpha^-(\D)
        }\\

        \inferrule[]{}{
            \Omega_\alpha^-(bool) = \emptyset
        }\\

        \inferrule[]{}{
            \Omega_\alpha^-(\op) = \emptyset
        }\\

        \inferrule[]{}{
            \Omega_\alpha^-(\delta) = \emptyset
        }\\

        \inferrule[]{}{
            \Omega_\alpha^-(\dirt_1 \union \dirt_2) = \Omega_\alpha^-(\dirt_1) + \Omega_\alpha^-(\dirt_2)
        }\\

        \inferrule[]{}{
            \Omega_\alpha^-(\rectype{A}) = \emptyset
        }\\

        \inferrule[]{}{
            \Omega_\alpha^-(\mu \beta . A) = \Omega^-_\beta(A)^*. \Omega_\alpha^-([\top / \beta]A)
        }
    \end{mathpar}
    \end{minipage}

    \end{framed}
    \end{center}
\caption{Encoding recursive types as type automata}\label{fig:automata:enc:rec}
\end{figure}

\section{Decoding}
\todo{explain decoding}

\begin{figure}[!htb]
    \begin{center}
    \begin{framed}
    \begin{minipage}[t]{0.95\columnwidth}
    \begin{mathpar}    
        (A_1^+, A_1^-) + (A_2^+, A_2^-) = (A_1^+ \union A_2^+, A_1^- \intersection A_2^-)\\
        (\C_1^+, \C_1^-) + (\C_2^+, \C_2^-) = (\C_1^+ \union \C_2^+, \C_1^- \intersection \C_2^-)\\

        (A_1^+, A_1^-) . (A_2^+, A_2^-) = \left \{
        \begin{tabular}{cr}
        $(\bot, \top)$ & if $(A_2^+, A_2^-) = (\bot, \top)$ \\
        \Big(
            \begin{tabular}{cr}
            $[A_2^+ / \unknowntp^+ , A_2^- / \unknowntp^-]A_1^+$, \\
            $[A_2^+ / \unknowntp^+ , A_2^- / \unknowntp^-]A_1^-$\\
            \end{tabular}
            \Big)  & otherwise \\
        \end{tabular}
        \right \}\\

        (\C_1^+, \C_1^-) . (\C_2^+, \C_2^-) = \left \{
        \begin{tabular}{cr}
        $(\bot \E \emptyset, \top \E \allops)$ & if $(\C_2^+, \C_2^-) = (\bot \E \emptyset, \top \E \allops)$ \\
        \Big(
            \begin{tabular}{cr}
            $[\C_2^+ / \unknowntp^+ \E \unknowndrttp^+, \C_2^- / \unknowntp^- \E \unknowndrttp^-]\C_1^+$, \\
            $[\C_2^+ / \unknowntp^+ \E \unknowndrttp^+ , \C_2^- / \unknowntp^- \E \unknowndrttp^-]\C_1^-$\\
            \end{tabular}
            \Big)  & otherwise \\
        \end{tabular}
        \right \}\\

        (\C_1^+, \C_1^-) . (A_2^+, A_2^-) = \left \{
        \begin{tabular}{cr}
        $(\bot \E \emptyset, \top \E \allops)$ & if $(A_2^+, A_2^-) = (\bot, \top)$ \\
        \Big(
            \begin{tabular}{cr}
            $[A_2^+ / \unknowntp^+ \E \unknowndrttp^+, A_2^- / \unknowntp^- \E \unknowndrttp^-]\C_1^+$, \\
            $[A_2^+ / \unknowntp^+ \E \unknowndrttp^+ , A_2^- / \unknowntp^- \E \unknowndrttp^-]\C_1^-$\\
            \end{tabular}
            \Big)  & otherwise \\
        \end{tabular}
        \right \}\\

        \inferrule[]{}{
            \dectype(\emptyset) = (\bot, \top) \\
            \dectype(\epsilon) = (\unknowntp, \unknowntp)
        }
    \end{mathpar}
    \end{minipage}
\end{framed}
\end{center}
\caption{Decoding type automata concat, union and kleene star into types}\label{fig:automata:dec}
\end{figure}

\begin{figure}[!htb]
    \begin{center}
    \begin{framed}
    \begin{minipage}[t]{0.475\columnwidth}
    \begin{mathpar}
        \inferrule[]{}{
            \dectype(\alpha^+) = (\alpha, \top)
        }\\

        \inferrule[]{}{
            \dectype(\functp^+) = (\top \to \bot, \top)
        }\\

        \inferrule[]{}{
            \dectype(d^+) = (\unknowntp \to \bot, \top)
        }\\

        \inferrule[]{}{
            \dectype(r^+) = (\top \to \unknowntp, \top)
        }\\

        \inferrule[]{}{
            \dectype(dh^+) = (\unknowntp \E \unknowndrttp \hto \bot, \top)
        }\\

        \inferrule[]{}{
            \dectype(rh^+) = (\top \hto \unknowntp \E \unknowndrttp, \top)
        }\\
        
        \inferrule[]{}{
            \dectype(\booltp^+) = (bool, \top)
        }\\
    
        \inferrule[]{}{
            \dectype(\dirttp^+) = (\bot \E \emptyset, \top)
        }\\

        \inferrule[]{}{
            \dectype(\optp{\op}^+) = (\bot \E \op, \top \E \allops)
        }\\

        \inferrule[]{}{
            \dectype(t^+) = (\unknowntp \E \emptyset, \top \E \allops)
        }\\
    
        \inferrule[]{}{
            \dectype(e^+) = (\bot \E \unknowndrttp, \top \E \allops)
        }
        
    \end{mathpar}
    \end{minipage}
    \begin{minipage}[t]{0.475\columnwidth}
    \begin{mathpar}
        \inferrule[]{}{
            \dectype(\alpha^-) = (\bot, \alpha)
        }\\

        \inferrule[]{}{
            \dectype(\functp^-) = (\bot, \top \to \bot)
        }\\

        \inferrule[]{}{
            \dectype(d^-) = (\bot, \unknowntp \to \bot)
        }\\

        \inferrule[]{}{
            \dectype(r^-) = (\bot, \top \to \unknowntp)
        }\\

        \inferrule[]{}{
            \dectype(dh^-) = (\bot, \unknowntp \hto \bot)
        }\\

        \inferrule[]{}{
            \dectype(rh^-) = (\bot, \top \hto \unknowntp)
        }\\
        
        \inferrule[]{}{
            \dectype(\booltp^-) = (\bot, bool)
        }\\
    
        \inferrule[]{}{
            \dectype(\dirttp^-) = (\bot, \bot \E \emptyset)
        }\\

        \inferrule[]{}{
            \dectype(\optp{\op}^-) = (\bot, \bot \E \op)
        }\\

        \inferrule[]{}{
            \dectype(t^-) = (\bot, \unknowntp \E \emptyset)
        }\\
    
        \inferrule[]{}{
            \dectype(e^-) = (\bot, \bot \E \unknowndrttp)
        }
    \end{mathpar}
    \end{minipage}

    \end{framed}
    \end{center}
\caption{Decoding type automata into types}\label{fig:automata:dec}
\end{figure}